src3.0/Transforms/die.v
@@ -10,6 +10,7 @@ Require Import primitives.
 Require Import program_sim.
 Require Import palloca_props.
 Require Import top_sim.
+Require Import trans_tactic.
 
 Definition pure_cmd (c:cmd) : Prop :=
 match c with
@@ -31,41 +32,18 @@ Record DIInfo := mkDIInfo {
 }.
 
 Definition fdef_simulation (diinfo: DIInfo) f1 f2 : Prop :=
-  if (fdef_dec (DI_f diinfo) f1) then remove_fdef (DI_id diinfo) f1 = f2
-  else f1 = f2.
+RemoveSim.fdef_simulation (DI_f diinfo) (DI_id diinfo) f1 f2.
 
 Definition cmds_simulation (diinfo: DIInfo) (f1:fdef) cs1 cs2 : Prop :=
-  if (fdef_dec (DI_f diinfo) f1) then remove_cmds (DI_id diinfo) cs1 = cs2
-  else cs1 = cs2.
+RemoveSim.cmds_simulation (DI_f diinfo) (DI_id diinfo) f1 cs1 cs2.
 
 Definition block_simulation (diinfo: DIInfo) (f1:fdef) b1 b2 : Prop :=
-  if (fdef_dec (DI_f diinfo) f1) then remove_block (DI_id diinfo) b1 = b2
-  else b1 = b2.
-
-Lemma fdef_simulation__eq_fheader: forall dinfo f1 f2
-  (H: fdef_simulation dinfo f1 f2),
-  fheaderOfFdef f1 = fheaderOfFdef f2.
-Proof.
-  unfold fdef_simulation.
-  intros.
-  destruct (fdef_dec (DI_f dinfo) f1); inv H; auto.
-    destruct (DI_f dinfo) as [fh b]; simpl; auto.
-Qed.
-
-Lemma fdef_simulation__det_right: forall dinfo f f1 f2,
-  fdef_simulation dinfo f f1 ->
-  fdef_simulation dinfo f f2 ->
-  f1 = f2.
-Proof.
-  unfold fdef_simulation.
-  intros.
-  destruct_if; congruence.
-Qed.
+RemoveSim.block_simulation (DI_f diinfo) (DI_id diinfo) f1 b1 b2.
 
 Definition Fsim (diinfo: DIInfo) := mkFunSim 
 (fdef_simulation diinfo)
-(fdef_simulation__eq_fheader diinfo)
-(fdef_simulation__det_right diinfo)
+(RemoveSim.fdef_simulation__eq_fheader (DI_f diinfo) (DI_id diinfo))
+(RemoveSim.fdef_simulation__det_right (DI_f diinfo) (DI_id diinfo))
 .
 
 Definition products_simulation (diinfo: DIInfo) Ps1 Ps2 : Prop :=
@@ -121,26 +99,360 @@ match (St1, St2) with
     gl1 = gl2 /\ fs1 = fs2 /\ M1 = M2
 end.
 
-Definition removable_State (diinfo: DIInfo) (St:@Opsem.State DGVs) : Prop :=
-match St with
-| Opsem.mkState
-    (Opsem.mkEC f b (c :: cs) tmn lc als::_) _ =>
-    if (fdef_dec (DI_f diinfo) f) then
-      if (id_dec (DI_id diinfo) (getCmdLoc c)) then True else False
-    else False
-| _ => False
+Definition value_doesnt_use_did dinfo F v :=
+  conditional_used_in_value (DI_f dinfo) F (DI_id dinfo) v.
+
+(* go to *)
+Ltac destruct_dec :=
+match goal with
+| |- context [id_dec ?b ?a] =>
+  destruct (id_dec b a); subst; try congruence; auto
+| _: context [id_dec ?b ?a] |- _ =>
+  destruct (id_dec b a); subst; try congruence; auto
+| _ : context [productInModuleB_dec ?p1 ?p2] |- _ =>
+  destruct (productInModuleB_dec p1 p2); try congruence
 end.
 
-Lemma removable_State_dec : forall diinfo St,
-  removable_State diinfo St \/ ~ removable_State diinfo St.
+Lemma simulation__getOperandValue : forall dinfo lc lc2 los nts  
+  gl F v (Hprop: value_doesnt_use_did dinfo F v)
+  (Hrsim: reg_simulation dinfo F lc lc2),
+  Opsem.getOperandValue (los,nts) v lc gl = 
+    Opsem.getOperandValue (los,nts) v lc2 gl.
 Proof.
-  destruct St.
-  destruct ECS as [|[]]; auto.
-  destruct CurCmds; auto.
-  simpl.
-  destruct (fdef_dec (DI_f diinfo) CurFunction); auto.
-  destruct (id_dec (DI_id diinfo) (getCmdLoc c)); auto.
+  intros.
+  unfold reg_simulation in Hrsim.
+  unfold value_doesnt_use_did in Hprop.
+  destruct (fdef_dec (DI_f dinfo) F); subst; auto.
+    unfold Opsem.getOperandValue in *.
+    destruct v; auto.
+      destruct Hprop as [Hprop | Hprop]; try congruence.
+      simpl in Hprop.
+      destruct (id_dec (DI_id dinfo) id5); subst; auto.  
+      destruct_dec. inv Hprop.
 Qed.
+
+Definition phis_simulation (dinfo: DIInfo) (f1:fdef) ps1 ps2 : Prop :=
+RemoveSim.phis_simulation (DI_f dinfo) (DI_id dinfo) f1 ps1 ps2.
+
+Lemma phis_simulation_inv: forall dinfo F ps1 ps2 l1 cs1 tmn1
+  (HBinF: blockInFdefB (block_intro l1 ps1 cs1 tmn1) F = true),
+  uniqFdef F ->
+  phis_simulation dinfo F ps1 ps2 -> ps1 = ps2.
+Proof.
+  intros.
+  eapply RemoveSim.phis_simulation_inv; eauto 1.
+    intro. subst. admit. (* phicannot be removed *)
+Qed.
+
+(* regsim can also be generalized *)
+Lemma reg_simulation_update_non_dead: forall dinfo F lc1 lc2 id0 gvs,
+  DI_f dinfo <> F \/ DI_id dinfo <> id0 ->
+  reg_simulation dinfo F lc1 lc2 ->
+  reg_simulation dinfo F (updateAddAL (GVsT DGVs) lc1 id0 gvs)
+    (updateAddAL (GVsT DGVs) lc2 id0 gvs).
+Proof.
+  unfold reg_simulation.
+  intros.
+  destruct (fdef_dec (DI_f dinfo) F); subst; intros; auto.
+    assert (J:=@H0 i0). clear H0.
+    destruct H as [H | H]; try congruence.
+    destruct (id_dec id0 i0); subst.
+      rewrite lookupAL_updateAddAL_eq; auto.
+      rewrite lookupAL_updateAddAL_eq; auto.
+
+      rewrite <- lookupAL_updateAddAL_neq; auto.
+      rewrite <- lookupAL_updateAddAL_neq; auto.
+Qed.
+
+Lemma getIncomingValuesForBlockFromPHINodes_rsim : forall los nts B1 B2 gl F
+  lc1' dinfo lc2' ps
+  (Hnuse: DI_f dinfo <> F \/ ~ In (DI_id dinfo) (getPhiNodesIDs ps))
+  (Hnuse': DI_f dinfo <> F \/
+           fold_left
+             (fun (re : bool) (p : phinode) => re || used_in_phi (DI_id dinfo) p)
+           ps false = false)
+  (l3 l0:list (id * GVsT DGVs))
+  (HeqR0 : Opsem.getIncomingValuesForBlockFromPHINodes (los,nts) ps B1 gl lc1' =
+           ret l3)
+  (Hbsim2 : block_simulation dinfo F B1 B2)
+  (Hrsim : reg_simulation dinfo F lc1' lc2')
+  (HeqR : Opsem.getIncomingValuesForBlockFromPHINodes (los,nts) ps B2 gl lc2' =
+          ret l0),
+  reg_simulation dinfo F (Opsem.updateValuesForNewBlock l3 lc1')
+     (Opsem.updateValuesForNewBlock l0 lc2').
+Proof.
+  induction ps as [|[i0 ? l0]]; simpl; intros.
+    uniq_result. simpl. auto.
+
+    inv_mbind'. symmetry_ctx. simpl.
+    assert (DI_f dinfo <> F \/ DI_id dinfo <> i0) as J1.
+      clear - Hnuse.
+      destruct Hnuse as [Hnuse | Hnuse]; auto.
+    assert (reg_simulation dinfo F
+             (Opsem.updateValuesForNewBlock l1 lc1')
+             (Opsem.updateValuesForNewBlock l2 lc2')) as J2.
+      assert (DI_f dinfo <> F \/ ~ In (DI_id dinfo) (getPhiNodesIDs ps)) as J3.
+        clear - Hnuse.
+        destruct Hnuse as [Hnuse | Hnuse]; auto.
+      assert (DI_f dinfo <> F \/
+              fold_left
+                (fun (re : bool) (p : phinode) =>
+                  re || used_in_phi (DI_id dinfo) p)
+                 ps false = false) as J4.
+        clear - Hnuse'.
+        destruct Hnuse' as [Hnuse' | Hnuse']; auto.
+        right.
+        assert (J:=Hnuse').
+        apply fold_left_eq in J.
+          rewrite J in Hnuse'. auto.
+          intros. apply orb_false_iff in H. destruct H; auto.
+      apply IHps; auto.
+    erewrite RemoveSim.block_simulation__getValueViaBlockFromValuels in HeqR3; 
+      eauto.
+    erewrite simulation__getOperandValue in HeqR0; eauto.
+      repeat uniq_result. 
+      apply reg_simulation_update_non_dead; auto.
+
+      destruct B2. simpl in HeqR3.
+      assert (DI_f dinfo <> F \/ used_in_list_value_l (DI_id dinfo) l0 = false)
+        as J3.
+        clear - Hnuse'.
+        destruct Hnuse' as [Hnuse' | Hnuse']; auto.
+        right.
+        apply fold_left_eq in Hnuse'; auto.
+          intros. apply orb_false_iff in H. destruct H; auto.
+      eapply conditional_used_in_getValueViaLabelFromValuels; eauto 1.
+Qed.
+
+Lemma switchToNewBasicBlock_rsim : forall los nts l1 l2 ps cs1 cs2 tmn1 tmn2 B1 
+  B2 gl lc1 lc2 F dinfo lc1' lc2' 
+  (Hnuse': DI_f dinfo <> F \/
+           fold_left
+             (fun (re : bool) (p : phinode) => re || used_in_phi (DI_id dinfo) p)
+           ps false = false)
+  (Huniq: uniqFdef F)
+  (HBinF: blockInFdefB (block_intro l1 ps cs1 tmn1) F = true)
+  (H23 : @Opsem.switchToNewBasicBlock DGVs (los,nts)
+          (block_intro l1 ps cs1 tmn1) B1 gl lc1' =
+         ret lc1)
+  (Hbsim2 : block_simulation dinfo F B1 B2)
+  (Hrsim: reg_simulation dinfo F lc1' lc2')
+  (H2 : Opsem.switchToNewBasicBlock (los,nts)
+         (block_intro l2 ps cs2 tmn2) B2 gl lc2' =
+        ret lc2), reg_simulation dinfo F lc1 lc2.
+Proof.
+  intros.
+  unfold Opsem.switchToNewBasicBlock in *. simpl in *.
+  inv_mbind'. symmetry_ctx.
+  eapply getIncomingValuesForBlockFromPHINodes_rsim; eauto.
+    admit. (* phi isnt dead *)
+Qed.
+
+Definition list_value_doesnt_use_did dinfo F idxs :=
+  conditional_used_in_list_value (DI_f dinfo) F (DI_id dinfo) idxs.
+
+Definition params_dont_use_did dinfo F (ps:params) :=
+  conditional_used_in_params (DI_f dinfo) F (DI_id dinfo) ps.
+
+Lemma reg_simulation__params2GVs: forall dinfo F lc1 lc2 gl
+  los nts (Hrsim: reg_simulation dinfo F lc1 lc2) 
+  lp (Hnuse: params_dont_use_did dinfo F lp),
+  Opsem.params2GVs (los,nts) lp lc1 gl =
+    Opsem.params2GVs (los,nts) lp lc2 gl.
+Proof.
+  induction lp as [|[]]; intros; subst; simpl in *.
+    auto.
+
+    assert (params_dont_use_did dinfo F lp
+             /\ value_doesnt_use_did dinfo F v) as J.
+      unfold params_dont_use_did in Hnuse. unfold params_dont_use_did.
+      unfold value_doesnt_use_did.
+      destruct (fdef_dec (DI_f dinfo) F); subst; auto.
+      destruct Hnuse as [Hnuse | Hnuse]; try congruence.
+      simpl in Hnuse. assert (J:=Hnuse).
+      apply fold_left_eq in Hnuse.
+        rewrite Hnuse in J.
+        binvf Hnuse as J1 J2.
+        split; right; auto.
+
+        intros. destruct b.
+        binvf H as J1 J2. auto.
+    destruct J as [J1 J2]. 
+    erewrite simulation__getOperandValue; eauto.
+    rewrite IHlp; auto.
+Qed.
+
+Definition args_dont_use_did dinfo F (la:list (typ * attributes * id)) :=
+  conditional_used_in_args (DI_f dinfo) F (DI_id dinfo) la.
+
+Lemma reg_simulation__initializeFrameValues: forall dinfo fa0 rt0 fid0 va0
+    TD lb la2 la1 (gvs:list (GVsT DGVs)) lc1 lc2 lc1' lc2'
+  (Hnuse: args_dont_use_did dinfo
+            (fdef_intro (fheader_intro fa0 rt0 fid0 (la1++la2) va0) lb) la2),
+  reg_simulation dinfo 
+    (fdef_intro (fheader_intro fa0 rt0 fid0 (la1++la2) va0) lb) lc1 lc2 ->
+  Opsem._initializeFrameValues TD la2 gvs lc1 = ret lc1' ->
+  Opsem._initializeFrameValues TD la2 gvs lc2 = ret lc2' ->
+  reg_simulation dinfo 
+    (fdef_intro (fheader_intro fa0 rt0 fid0 (la1++la2) va0) lb) lc1' lc2'.
+Proof.
+  induction la2 as [|[[]]]; simpl; intros.
+    uniq_result. auto.
+
+    assert (args_dont_use_did dinfo
+       (fdef_intro
+          (fheader_intro fa0 rt0 fid0 ((la1 ++ [(t, a, i0)]) ++ la2) va0) lb)
+       la2) as J.
+      unfold args_dont_use_did. unfold args_dont_use_did in Hnuse.
+      simpl_env. simpl_env in Hnuse.
+      destruct Hnuse as [Hnuse | Hnuse]; auto.
+      right.
+      intros.
+      eapply Hnuse; simpl; eauto.
+
+    assert (DI_f dinfo <>
+      fdef_intro (fheader_intro fa0 rt0 fid0 (la1 ++ (t, a, i0) :: la2) va0) lb\/
+      DI_id dinfo <> i0) as J'.
+      unfold args_dont_use_did in Hnuse.
+      destruct Hnuse as [Hnuse | Hnuse]; auto.
+      right.
+      eapply Hnuse; simpl; eauto.
+
+    rewrite_env ((la1 ++ [(t, a, i0)]) ++ la2) in H.
+    destruct gvs; inv_mbind''; symmetry_ctx.
+      eapply IHla2 in H; eauto.
+        apply reg_simulation_update_non_dead; auto.
+        simpl_env in *. auto.
+
+      eapply IHla2 in H; eauto.
+        apply reg_simulation_update_non_dead; auto.
+        simpl_env in *. auto.
+Qed.
+
+Lemma reg_simulation_nil: forall dinfo F, reg_simulation dinfo F nil nil.
+Proof.
+  unfold reg_simulation.
+  intros.
+  destruct (fdef_dec (DI_f dinfo) F); subst; auto.
+Qed.
+
+Lemma reg_simulation__initLocals: forall dinfo F lc1 lc2 lp gl gvs1 gvs2 lc1'
+  lc2' la los nts fa0 rt0 fid0 va0 lb 
+  (Hnuse: params_dont_use_did dinfo F lp)
+  (Hnuse': args_dont_use_did dinfo
+            (fdef_intro (fheader_intro fa0 rt0 fid0 la va0) lb) la),
+  reg_simulation dinfo F lc1 lc2 ->
+  Opsem.params2GVs (los,nts) lp lc1 gl = ret gvs1 ->
+  Opsem.params2GVs (los,nts) lp lc2 gl = ret gvs2 ->
+  Opsem.initLocals (los,nts) la gvs1 = ret lc1' ->
+  Opsem.initLocals (los,nts) la gvs2 = ret lc2' ->
+  reg_simulation dinfo 
+    (fdef_intro (fheader_intro fa0 rt0 fid0 la va0) lb) lc1' lc2'.
+Proof.
+  intros.
+  erewrite reg_simulation__params2GVs in H0; eauto. 
+  uniq_result.
+  unfold Opsem.initLocals in *.
+  rewrite_env (nil++la).
+  eapply reg_simulation__initializeFrameValues; eauto.
+  apply reg_simulation_nil; auto.
+Qed.
+
+Ltac destruct_ctx_other :=
+match goal with
+| Hwfcfg : OpsemPP.wf_Config
+            {|
+            OpsemAux.CurSystem := _;
+            OpsemAux.CurTargetData := ?TD;
+            OpsemAux.CurProducts := _;
+            OpsemAux.Globals := _;
+            OpsemAux.FunTable := _
+             |},
+  Hwfpp : OpsemPP.wf_State
+            {|
+            OpsemAux.CurSystem := _;
+            OpsemAux.CurTargetData := ?TD;
+            OpsemAux.CurProducts := _;
+            OpsemAux.Globals := _;
+            OpsemAux.FunTable := _
+             |} _,
+  Hsim : State_simulation _ _ _ _ _ ?Cfg2 ?St2 ,
+  Hop2 : Opsem.sInsn _ _ _ _ |- _ =>
+  destruct TD as [los nts];
+  destruct Hwfcfg as [_ [Hwfg [HwfSystem HmInS]]];
+  destruct Hwfpp as
+    [_ [
+     [Hreach1 [HBinF1 [HFinPs1 _]]]
+     [ _ HwfCall'
+     ]]
+    ]; subst;
+  destruct Cfg2 as [S2 TD2 Ps2 gl2 fs2];
+  destruct St2 as [ECs2 M2];
+  simpl in Hsim;
+  destruct Hsim as [EQ1 [Hpsim [Hstksim [EQ2 [EQ3 Hmsim]]]]]; subst;
+  destruct ECs2 as [|[F2 B2 cs2 tmn2 lc2 als2] ECs2]; tinv Hstksim;
+  destruct Hstksim as [Hecsim Hstksim];
+  unfold EC_simulation in Hecsim;
+  destruct Hecsim as
+      [Hfsim2 [Heq1 [Halsim2 [Hbsim2
+        [Heq3 [Heq4 [Hlcsim2 Hcssim2]]]]]]]; subst;
+  assert (Heq3':=Heq3); destruct Heq3' as [l3 [ps1 [cs11 Heq3']]]; subst
+end.
+
+Ltac destruct_ctx_return :=
+match goal with
+| Hwfcfg : OpsemPP.wf_Config
+            {|
+            OpsemAux.CurSystem := _;
+            OpsemAux.CurTargetData := ?TD;
+            OpsemAux.CurProducts := _;
+            OpsemAux.Globals := _;
+            OpsemAux.FunTable := _
+             |},
+  Hwfpp : OpsemPP.wf_State
+            {|
+            OpsemAux.CurSystem := _;
+            OpsemAux.CurTargetData := ?TD;
+            OpsemAux.CurProducts := _;
+            OpsemAux.Globals := _;
+            OpsemAux.FunTable := _
+             |} _,
+  Hsim : State_simulation _ _ _ _ _ ?Cfg2 ?St2 ,
+  Hop2 : Opsem.sInsn _ _ _ _ |- _ =>
+  destruct TD as [los nts];
+  destruct Hwfcfg as [_ [Hwfg [HwfSystem HmInS]]];
+  destruct Hwfpp as
+    [_ [
+     [Hreach1 [HBinF1 [HFinPs1 _]]]
+     [
+       [
+         [Hreach2 [HBinF2 [HFinPs2 _]]]
+         _
+       ]
+       HwfCall'
+     ]]
+    ]; subst;
+  destruct Cfg2 as [S2 TD2 Ps2 gl2 fs2];
+  destruct St2 as [ECs2 M2];
+  simpl in Hsim;
+  destruct Hsim as [EQ1 [Hpsim [Hstksim [EQ2 [EQ3 Hmsim]]]]]; subst;
+  destruct ECs2 as [|[F2 B2 cs2 tmn2 lc2 als2] ECs2]; tinv Hstksim;
+  destruct Hstksim as [Hecsim Hstksim];
+  destruct ECs2 as [|[F3 B3 cs3 tmn3 lc3 als3] ECs2]; tinv Hstksim;
+  destruct Hstksim as [Hecsim' Hstksim];
+  unfold EC_simulation in Hecsim;
+  destruct Hecsim as
+      [Hfsim2 [Heq1 [Halsim2 [Hbsim2
+        [Heq3 [Heq4 [Hlcsim2 Hcssim2]]]]]]]; subst;
+  destruct Hecsim' as
+      [Hfsim2' [Heq1' [Halsim2' [Hbsim2'
+        [Heq3' [Heq4' [Hlcsim2' Hcssim2']]]]]]]; subst;
+  apply RemoveSim.cmds_simulation_nil_inv in Hcssim2; subst;
+  wfCall_inv
+end.
+
+Definition removable_State (dinfo: DIInfo) (St:@Opsem.State DGVs) : Prop :=
+RemoveSim.removable_State (DI_f dinfo) (DI_id dinfo) St.
 
 Lemma die_is_sim : forall diinfo Cfg1 St1 Cfg2 St2
   (Hwfpp: OpsemPP.wf_State Cfg1 St1)
@@ -152,6 +464,395 @@ Lemma die_is_sim : forall diinfo Cfg1 St1 Cfg2 St2
      (Hop2: Opsem.sInsn Cfg2 St2 St2' tr2)
      (Hop1: Opsem.sInsn Cfg1 St1 St1' tr1),
      State_simulation diinfo Cfg1 St1' Cfg2 St2' /\ tr1 = tr2).
+Proof.
+
+Local Opaque inscope_of_tmn inscope_of_cmd.
+
+  intros.
+  split; intros.
+(*
+Case "removable state". eapply dae_is_sim_removable_state; eauto.
+
+Case "unremovable state".
+  apply RemoveSim.not_removable_State_inv in Hnrem.
+  (sInsn_cases (destruct Hop1) SCase).
+
+SCase "sReturn".
+Focus.
+
+  destruct_ctx_return.
+  assert (PI_f pinfo <> F' \/ PI_id pinfo <> getCmdLoc (insn_call i0 n c t0 v0 v p))
+    as Hneq.
+    WF_PhiInfo_spec10_tac.
+  apply RemoveSim.cmds_simulation_nelim_cons_inv in Hcssim2'; auto.
+  destruct Hcssim2' as [cs3' [Heq Hcssim2']]; subst;
+  inv Hop2;
+  uniq_result.
+  eapply free_allocas_return_sim in Hmsim; eauto.
+  exists mi.
+  repeat_solve.
+    eapply returnUpdateLocals_als_simulation; eauto.
+
+    eapply returnUpdateLocals_reg_simulation with (lc:=lc);
+      eauto using mem_simulation__wf_sb_sim;
+      try solve [get_wf_value_for_simop'; eauto].
+      eapply conditional_used_in_fdef__used_in_tmn_value; eauto; simpl; auto.
+
+Unfocus.
+
+SCase "sReturnVoid".
+Focus.
+  destruct_ctx_return.
+  assert (PI_f pinfo <> F' \/ PI_id pinfo <> getCmdLoc (insn_call i0 n c t0 v0 v p))
+    as Hneq.
+    WF_PhiInfo_spec10_tac.
+  apply RemoveSim.cmds_simulation_nelim_cons_inv in Hcssim2'; auto.
+  destruct Hcssim2' as [cs3' [Heq Hcssim2']]; subst;
+  inv Hop2;
+  uniq_result.
+  eapply free_allocas_return_void_sim in Hmsim; eauto.
+  exists mi.
+  repeat_solve.
+
+Unfocus.
+
+SCase "sBranch".
+Focus.
+  destruct_ctx_other.
+  apply RemoveSim.cmds_simulation_nil_inv in Hcssim2; subst.
+  inv Hop2.
+  uniq_result.
+
+  assert (block_simulation pinfo F (block_intro l' ps' cs' tmn')
+           (block_intro l'0 ps'0 cs'0 tmn'0)) as Hbsim.
+    destruct Hmsim as [_ [_ Hwf_mi]].
+    eapply simulation__getOperandValue in Hlcsim2;
+      try solve [get_wf_value_for_simop'; eauto 2].
+      erewrite simulation__isGVZero in H1; eauto.
+      clear - H22 H1 Hfsim2.
+      destruct (isGVZero (los, nts) c0); 
+        eapply RemoveSim.fdef_sim__block_sim; eauto.
+
+      eapply conditional_used_in_fdef__used_in_tmn_value; eauto; simpl; auto.
+
+  assert (Hbsim':=Hbsim).
+  apply RemoveSim.block_simulation_inv in Hbsim'.
+  destruct Hbsim' as [Heq1 [Hpssim' [Hcssim' Heq5]]]; subst.
+
+  assert (uniqFdef F) as Huniq. eauto using wf_system__uniqFdef.
+  assert (blockInFdefB (block_intro l'0 ps' cs' tmn'0) F) as HBinF1'.
+    solve_blockInFdefB.
+  eapply phis_simulation_inv in Hpssim'; eauto 2.
+  subst.
+
+  assert (reg_simulation pinfo mi F lc' lc'0) as Hlcsim2'.
+    assert (HBinF1'':=HBinF1').
+    eapply wf_system__blockInFdefB__wf_block in HBinF1''; eauto.     
+    inv HBinF1''.
+    eapply switchToNewBasicBlock_rsim in Hbsim2;
+      eauto using mem_simulation__wf_sb_sim, conditional_used_in_fdef__used_in_phis.
+  assert (als_simulation pinfo mi F lc' als als2) as Halsim2'.
+    eapply switchToNewBasicBlock_asim; eauto.
+  exists mi.
+  repeat_solve.
+    exists l'0. exists ps'0. exists nil. auto.
+    exists l'0. exists ps'0. exists nil. auto.
+
+    destruct Hmsim as [J1 [J2 J3]].
+    split; auto.
+    split; auto.
+      intros blk J.
+      apply J2.
+      intro J4. apply J.
+      simpl.
+      eapply switchToNewBasicBlock_isnt_alloca_in_ECs; eauto; simpl; eauto.
+Unfocus.
+
+SCase "sBranch_uncond".
+Focus.
+  destruct_ctx_other.
+  apply RemoveSim.cmds_simulation_nil_inv in Hcssim2; subst.
+  inv Hop2.
+  uniq_result.
+
+  assert (block_simulation pinfo F (block_intro l' ps' cs' tmn')
+           (block_intro l'0 ps'0 cs'0 tmn'0)) as Hbsim.
+    eapply RemoveSim.fdef_sim__block_sim; eauto.
+  assert (Hbsim':=Hbsim).
+  apply RemoveSim.block_simulation_inv in Hbsim'.
+  destruct Hbsim' as [Heq1 [Hpssim' [Hcssim' Heq5]]]; subst.
+
+  assert (uniqFdef F) as Huniq. eauto using wf_system__uniqFdef.
+  assert (blockInFdefB (block_intro l'0 ps' cs' tmn'0) F) as HBinF1'.
+    solve_blockInFdefB.
+  eapply phis_simulation_inv in Hpssim'; eauto 2.
+  subst.
+
+  assert (reg_simulation pinfo mi F lc' lc'0) as Hlcsim2'.
+    assert (HBinF1'':=HBinF1').
+    eapply wf_system__blockInFdefB__wf_block in HBinF1''; eauto.     
+    inv HBinF1''.
+    eapply switchToNewBasicBlock_rsim in Hbsim2;
+      eauto using mem_simulation__wf_sb_sim, conditional_used_in_fdef__used_in_phis.
+  assert (als_simulation pinfo mi F lc' als als2) as Halsim2'.
+    eapply switchToNewBasicBlock_asim; eauto.
+  exists mi.
+  repeat_solve.
+    exists l'0. exists ps'0. exists nil. auto.
+    exists l'0. exists ps'0. exists nil. auto.
+
+    destruct Hmsim as [J1 [J2 J3]].
+    split; auto.
+    split; auto.
+      intros blk J.
+      apply J2.
+      intro J4. apply J. simpl.
+      eapply switchToNewBasicBlock_isnt_alloca_in_ECs; eauto; simpl; eauto.
+Unfocus.
+
+SCase "sBop". abstract (destruct_ctx_other; dse_is_sim_common_case).
+SCase "sFBop". abstract (destruct_ctx_other; dse_is_sim_common_case).
+SCase "sExtractValue". abstract (destruct_ctx_other; dse_is_sim_common_case).
+SCase "sInsertValue". abstract (destruct_ctx_other; dse_is_sim_common_case).
+SCase "sMalloc".
+  abstract (destruct_ctx_other;
+  apply RemoveSim.cmds_simulation_nelim_cons_inv in Hcssim2; simpl; auto;
+  destruct Hcssim2 as [cs3' [Heq Hcssim2]]; subst;
+  inv Hop2; uniq_result;
+  eapply simulation__getOperandValue with (lc2:=lc2) in H0;
+    try simulation__getOperandValue_tac1;
+  eapply mem_simulation__malloc in Hmsim; eauto 2; simpl in Hmsim;
+  destruct Hmsim as [mi' [Hmsim [Hinc [Hprop1 Hprop2]]]];
+  exists mi';
+  repeat_solve; try solve [
+    eapply als_simulation__malloc; eauto | 
+    eapply reg_simulation__malloc; eauto |
+    eapply inject_incr__preserves__ECs_simulation; 
+      try solve [eauto | eapply malloc__isnt_alloca_in_ECs; eauto] |
+    eapply OpsemAux.inject_incr__preserves__ftable_simulation; eauto
+  ]).
+
+SCase "sFree".
+  abstract (destruct_ctx_other;
+  apply RemoveSim.cmds_simulation_nelim_cons_inv in Hcssim2; auto;
+  destruct Hcssim2 as [cs3' [Heq Hcssim2]]; subst;
+  inv Hop2; uniq_result;
+  eapply simulation__getOperandValue with (lc2:=lc2) in H;
+    try simulation__getOperandValue_tac1;
+  eapply mem_simulation__free in Hmsim; eauto 2;
+  exists mi;
+  repeat_solve).
+
+SCase "sAlloca".
+  abstract (destruct_ctx_other;
+  apply RemoveSim.cmds_simulation_nelim_cons_inv in Hcssim2; simpl; auto;
+  destruct Hcssim2 as [cs3' [Heq Hcssim2]]; subst;
+  inv Hop2; uniq_result;
+  eapply simulation__getOperandValue with (lc2:=lc2) in H0;
+    try simulation__getOperandValue_tac1;
+  eapply mem_simulation__malloc in Hmsim; eauto 2; simpl in Hmsim;
+  destruct Hmsim as [mi' [Hmsim [Hinc [Hprop1 Hprop2]]]];
+  exists mi';
+  repeat_solve; try solve [
+    eapply als_simulation__alloca; eauto | 
+    eapply reg_simulation__malloc; eauto |
+    eapply inject_incr__preserves__ECs_simulation; 
+      try solve [eauto | eapply malloc__isnt_alloca_in_ECs; eauto] |
+    eapply OpsemAux.inject_incr__preserves__ftable_simulation; eauto
+  ]).
+
+SCase "sLoad".
+  abstract (destruct_ctx_other;
+  apply RemoveSim.cmds_simulation_nelim_cons_inv in Hcssim2; simpl; auto;
+  destruct Hcssim2 as [cs3' [Heq Hcssim2]]; subst;
+  inv Hop2; uniq_result;
+  exists mi;
+  repeat_solve; try solve [
+    apply als_simulation_update_lc; auto |
+    apply reg_simulation_update_non_palloca; try solve [
+      auto |
+      eapply simulation__mload; try solve [
+        eauto 2 using mem_simulation__wf_sb_sim |
+        simulation__getOperandValue_tac2
+      ]
+    ] |
+    eapply mem_simulation__update_non_palloca; eauto; simpl; eauto
+  ]).
+
+SCase "sStore".
+  abstract (destruct_ctx_other;
+  apply RemoveSim.cmds_simulation_nelim_cons_inv in Hcssim2; auto;
+  destruct Hcssim2 as [cs3' [Heq Hcssim2]]; subst;
+  inv Hop2; uniq_result;
+  exists mi;
+  repeat_solve; try solve [
+    simpl; eapply simulation__mstore; try solve [
+      eauto 2 using mem_simulation__wf_sb_sim |
+      eapply simulation__getOperandValue; eauto using mem_simulation__wf_sb_sim;
+        try solve [eapply conditional_used_in_fdef__used_in_cmd_value;
+                     eauto using in_middle; simpl; auto |
+                   get_wf_value_for_simop; eauto]
+    ]
+  ]).
+
+SCase "sGEP". abstract (destruct_ctx_other; dse_is_sim_common_case).
+SCase "sTrunc". abstract (destruct_ctx_other; dse_is_sim_common_case).
+SCase "sExt". abstract (destruct_ctx_other; dse_is_sim_common_case).
+SCase "sCast". abstract (destruct_ctx_other; dse_is_sim_common_case).
+SCase "sIcmp". abstract (destruct_ctx_other; dse_is_sim_common_case).
+SCase "sFcmp". abstract (destruct_ctx_other; dse_is_sim_common_case).
+SCase "sSelect".
+  destruct_ctx_other.
+  apply RemoveSim.cmds_simulation_nelim_cons_inv in Hcssim2; simpl; auto;
+  destruct Hcssim2 as [cs3' [Heq Hcssim2]]; subst;
+  inv Hop2; uniq_result.
+  exists mi.
+  repeat_solve.
+    destruct (isGVZero (los,nts) c);
+      apply als_simulation_update_lc; auto.
+    erewrite simulation__isGVZero with (c':=c0);
+      simulation__getOperandValue_tac2.
+    destruct (isGVZero (los,nts) c0);
+      apply reg_simulation_update_non_palloca; eauto; try solve [
+        eapply simulation__getOperandValue;
+        eauto using mem_simulation__wf_sb_sim;
+        try solve [eapply conditional_used_in_fdef__used_in_cmd_value;
+                     eauto using in_middle; simpl; auto|
+                   get_wf_value_for_simop; eauto]
+      ].
+    destruct (isGVZero (los,nts) c);
+      eapply mem_simulation__update_non_palloca; eauto; simpl; eauto.
+
+SCase "sCall".
+  destruct_ctx_other.
+  assert (Hcssim2':=Hcssim2).
+  apply RemoveSim.cmds_simulation_nelim_cons_inv in Hcssim2; auto.
+  destruct Hcssim2 as [cs3' [Heq Hcssim2]]; subst.
+  inv Hop2; uniq_result.
+  SSCase "SCall".
+
+  assert (gv_inject mi fptr fptr0) as Hfptr_sim.
+    assert (exists t, wf_value S (module_intro los nts Ps) F fv t) as G.
+      assert (HBinF1':=HBinF1).
+      eapply wf_system__wf_cmd in HBinF1'; eauto using in_middle.     
+      inv HBinF1'. eauto.
+    destruct G.
+    simulation__getOperandValue_tac2.
+
+  assert (Hfsim1:=Hpsim).
+  eapply TopSim.lookupFdefViaPtr_inj__simulation in Hfsim1; eauto. 
+  simpl in Hfsim1.
+  assert (Hbsim1:=Hfsim1).
+  eapply RemoveSim.fdef_simulation__entry_block_simulation in Hbsim1; eauto.
+  assert (Hbsim1':=Hbsim1).
+  apply RemoveSim.block_simulation_inv in Hbsim1'.
+  destruct Hbsim1' as [Heq' [Hpsim1' [Hcsim1' Htsim1']]]; subst.
+  exists mi.
+    match goal with
+    | H1: OpsemAux.lookupFdefViaPtr _ _ _ = Some ?F,
+      _ : fdef_simulation _ ?F _ |- _ =>
+      apply OpsemAux.lookupFdefViaPtr_inv in H1;
+      eapply wf_system__uniqFdef in H1; eauto 2
+    end.
+  repeat_solve.
+    exists l'0. exists ps'. exists nil. auto.
+    exists l'0. exists ps'0. exists nil. auto.
+
+    apply RemoveSim.fdef_simulation_inv in Hfsim1.
+    destruct Hfsim1 as [Hfhsim1 Hbssim1].
+    inv Hfhsim1.
+    assert (HBinF1':=HBinF1).
+    eapply wf_system__wf_cmd in HBinF1'; eauto using in_middle.     
+    inv HBinF1'.
+    find_wf_value_list.  
+    eapply reg_simulation__initLocals; try solve [
+      eauto 2 using mem_simulation__wf_sb_sim, WF_PhiInfo__args_dont_use_pid |
+      eapply conditional_used_in_fdef__used_in_params; eauto 1
+    ].
+
+    destruct Hmsim as [Hmsim1 [Hmsim2 Hmsim3]].
+    split; auto.
+    split; auto.
+      intros blk J.
+      apply Hmsim2.
+      intro G. apply J.
+      unfold isnt_alloca_in_ECs in *.
+      intros. simpl in Hin.
+      destruct Hin as [Hin | Hin].
+        subst. simpl.
+        inv Hin. eapply WF_PhiInfo__isnt_alloca_in_EC; eauto.
+
+        apply G. simpl. auto.
+
+  SSCase "sExCall".
+
+  assert (gv_inject mi fptr fptr0) as Hfptr_sim.
+    assert (exists t, wf_value S (module_intro los nts Ps) F fv t) as G.
+      assert (HBinF1':=HBinF1).
+      eapply wf_system__wf_cmd in HBinF1'; eauto using in_middle.     
+      inv HBinF1'. eauto.
+    destruct G.
+    simulation__getOperandValue_tac2.
+
+  eapply TopSim.lookupFdefViaPtr_inj__simulation_l2r in H1; eauto.
+  uniq_result.
+
+SCase "sExCall".
+
+  destruct_ctx_other.
+  assert (Hcssim2':=Hcssim2).
+  apply RemoveSim.cmds_simulation_nelim_cons_inv in Hcssim2; auto.
+  destruct Hcssim2 as [cs3' [Heq Hcssim2]]; subst.
+  inv Hop2; uniq_result.
+
+  SSCase "SCall".
+
+  assert (gv_inject mi fptr fptr0) as Hfptr_sim.
+    assert (exists t, wf_value S (module_intro los nts Ps) F fv t) as G.
+      assert (HBinF1':=HBinF1).
+      eapply wf_system__wf_cmd in HBinF1'; eauto using in_middle.     
+      inv HBinF1'. eauto.
+    destruct G.
+    simulation__getOperandValue_tac2.
+
+  eapply TopSim.lookupFdefViaPtr_inj__simulation_r2l in H1; eauto.
+  uniq_result.
+
+  SSCase "sExCall".
+
+  assert (gv_inject mi fptr fptr0) as Hfptr_sim.
+    assert (exists t, wf_value S (module_intro los nts Ps) F fv t) as G.
+      assert (HBinF1':=HBinF1).
+      eapply wf_system__wf_cmd in HBinF1'; eauto using in_middle.     
+      inv HBinF1'. eauto.
+    destruct G.
+    simulation__getOperandValue_tac2.
+
+  eapply TopSim.lookupExFdecViaPtr_inj__simulation in Hfptr_sim; eauto.
+  uniq_result.
+
+  match goal with | H1 : fdec_intro _ _ = fdec_intro _ _ |- _ => inv H1 end.
+  assert (List.Forall2 (fun gv1 => fun gv2 => gv_inject mi gv1 gv2) gvss gvss0)
+    as Hparsim.
+    assert (HBinF1':=HBinF1).
+    eapply wf_system__wf_cmd in HBinF1'; eauto using in_middle.     
+    inv HBinF1'.
+    find_wf_value_list.  
+    eapply reg_simulation__params2GVs; try solve [
+      eauto 2 using mem_simulation__wf_sb_sim |
+      eapply conditional_used_in_fdef__used_in_params; eauto 1
+    ].
+  eapply callExternalFunction__mem_simulation in Hmsim; eauto.
+  destruct Hmsim as [EQ' [EQ [mi' [Hmsim [Hinc [J1 [J2 J3]]]]]]]; subst.
+  exists mi'.
+  repeat_solve.
+    eapply inject_incr__preserves__ECs_simulation; eauto.
+    eapply OpsemAux.inject_incr__preserves__ftable_simulation; eauto.
+
+Transparent inscope_of_tmn inscope_of_cmd.
+
+Qed.
+*)
 Admitted.
 
 Lemma s_genInitState__die_State_simulation:
@@ -226,7 +927,8 @@ Proof.
         apply OpsemPP.preservation in Hop1; auto.
       eapply die_is_sim in Hstsim; eauto.
       destruct Hstsim as [Hstsim1 Hstsim2].
-      destruct (@removable_State_dec diinfo IS1) as [Hrm | Hnrm].
+      destruct (@RemoveSim.removable_State_dec 
+          (DI_f diinfo) (DI_id diinfo) IS1) as [Hrm | Hnrm].
         eapply Hstsim1 in Hrm; eauto.
         destruct Hrm as [Hstsim EQ]; subst.
         admit. (* we should do induction on the measure of State_simulation *)
