src3.0/Transforms/program_sim.v
@@ -133,6 +133,22 @@ Proof.
     apply H1 in H7. unfold defined_program in H2. tauto. 
 Qed.
 
+Lemma val_inject__result_match: forall mi v1 v2
+  (Hinj: MoreMem.val_inject mi v1 v2), val_result_match v1 v2.
+Proof.
+  intros.
+  inv Hinj; constructor; auto.
+Qed.
+
+Lemma gv_inject__result_match: forall mi gvs1 gvs2
+  (Hinj:  genericvalues_inject.gv_inject mi gvs1 gvs2), result_match gvs1 gvs2.
+Proof.
+  unfold result_match.
+  induction 1; auto.
+    constructor; auto.
+      split; eauto using val_inject__result_match.
+Qed.
+
 Lemma program_sim__preserves__defined_program: forall P1 P2 main VarArgs
   (Hok: defined_program P2 main VarArgs) (Hsim: program_sim P1 P2 main VarArgs),
   defined_program P1 main VarArgs.
